theories/Lib.v
@@ -1,5 +1,5 @@
 (* Copyright 2023 Frédéric Besson <frederic.besson@inria.fr> *)
-Require Import Bool ZifyBool ZArith ZifyUint63 Uint63 Lia.
+Require Import Bool ZifyBool ZArith ZifyUint63 Uint63 Lia List.
 
 (* Some basic tactics and results *)
 
@@ -109,3 +109,129 @@ Ltac elim_match_comparison :=
        | Gt => _
        end] |- _ => let F := fresh in destruct X eqn:F
   end.
+
+(** lists *)
+Section FORALL2.
+  Context {A B:Type}.
+  Variable F : A -> B -> bool.
+
+  Fixpoint forall2b  (l1 : list A) (l2 : list B) : bool :=
+    match l1 , l2 with
+    | nil , nil => true
+    | e1::l1', e2::l2' => F e1 e2 && forall2b l1' l2'
+    | _      , _       => false
+    end.
+End FORALL2.
+
+Lemma forall2b_Forall2 : forall {A B: Type} (F : A -> B -> bool) l1 l2,
+    forall2b F l1 l2 = true <-> Forall2 (fun x y => F x y = true) l1 l2.
+Proof.
+  induction l1 ; simpl.
+  - destruct l2.
+    split ; auto.
+    intuition try congruence.
+    inv H.
+  - destruct l2.
+    split ; try discriminate.
+    intros. inv H.
+    rewrite andb_true_iff.
+    rewrite IHl1.
+    intuition. inv H ; auto.
+    inv H ;auto.
+Qed.
+
+
+Lemma Forall_rew : forall {T: Type} [P: T -> Prop] (l : list T),
+    Forall P l <-> match l with
+                   | nil => True
+                   | e::l => P e /\ Forall P l
+                   end.
+Proof.
+  destruct l.
+  - split ; auto.
+  - split ; intro.
+    inv H. tauto.
+    destruct H. constructor ; auto.
+Qed.
+
+(** [sublist] *)
+
+
+Inductive sublist {A: Type}: list A -> list A -> Prop :=
+| SUB_NIL : forall l, sublist nil l
+| SUB_CONS : forall l1 l2 a, sublist l1 l2 -> sublist l1 (a::l2)
+| SUB_CONS2: forall l1 l2 a, sublist l1 l2 -> sublist (a::l1) (a::l2).
+
+Lemma sublist_refl : forall {A: Type} (l: list A),
+    sublist l l.
+Proof.
+  induction l.
+  - constructor.
+  - apply SUB_CONS2. auto.
+Qed.
+
+Lemma sublist_forall : forall {A: Type} (P : A -> Prop) l1 l2,
+    Forall P l2 ->
+    sublist l1 l2 ->
+    Forall P l1.
+Proof.
+  intros.
+  induction H0.
+  constructor.
+  inv H.
+  tauto.
+  inv H.
+  constructor; auto.
+Qed.
+
+(* A naive Ltac [btauto] *)
+
+Ltac collect_boolean_vars E :=
+  match E with
+  | ?E1 || ?E2 => collect_bin E1 E2
+  | ?E1 && ?E2 => let e1 := collect_boolean_vars E1 in
+                  let e2 := collect_boolean_vars E2 in
+                  eval simpl in (e1 ++ e2)
+  |   _        => constr:(E::nil)
+  end
+    with collect_bin E1 E2 :=
+    let e1 := collect_boolean_vars E1 in
+    let e2 := collect_boolean_vars E2 in
+    eval simpl in (e1 ++ e2).
+
+
+
+Ltac simplify_bool :=
+  repeat match goal with
+  | |- context[?X && false] => rewrite (andb_false_r X)
+  | |- context[?X && true] => rewrite (andb_true_r X)
+  | |- context[?X || false] => rewrite (orb_false_r X)
+  | |- context[?X || true] => rewrite (orb_true_r X)
+  | |- context[negb true] =>  change (negb true) with false
+  | |- context[negb false] =>  change (negb false) with true
+  end.
+
+Ltac destruct_boolean L :=
+  match goal with
+  | |- true = false => gfail 0 "Not a tautolofy"
+  | |- false = true => gfail 0 "Not a tautolofy"
+  | |- _            =>
+      try reflexivity ;
+      lazymatch L with
+      | nil => reflexivity
+      | cons ?V ?L =>
+          match goal with
+          | |- context[V] => destruct V ; simplify_bool ; destruct_boolean L
+          | |-   _        => destruct_boolean L
+          end
+      end
+  end.
+
+
+Ltac btauto :=
+  match goal with
+  | |- @eq bool ?E1 ?E2 =>
+      let vars := collect_bin E1 E2  in
+      destruct_boolean vars
+  end.
+
