Ctauto.v
@@ -1,3 +1,0 @@
-Require Export Cdcl.Itauto.
-(** itauto is using the `classic` axiom if available *)
-#[export] Set Itauto Classic.
