theories/Clause.v
@@ -1,0 +1,355 @@
+(* Copyright 2023 Frédéric Besson <frederic.besson@inria.fr> *)
+Require Import Bool ZifyBool ZArith ZifyUint63 Uint63 Lia List.
+Require Import Cdcl.Lib Cdcl.Syntax Cdcl.Lit.
+
+(* A clause is a list of literals.
+   Section EvalList provides some results for manipulating lists *)
+
+Section EvalList.
+  Context {A: Type}.
+  Variable eval : A -> Prop.
+
+  Fixpoint eval_and_list  (l : list A) :=
+    match l with
+    | nil => True
+    | e :: nil => eval e
+    | e1 ::l   => eval e1 /\ eval_and_list l
+    end.
+
+  Fixpoint eval_and_list'  (l : list A) :=
+    match l with
+    | nil => True
+    | e1 ::l   => eval e1 /\ eval_and_list' l
+    end.
+
+  Lemma eval_and_list_eq : forall l,
+      eval_and_list l <-> eval_and_list' l.
+  Proof.
+    induction l ; simpl.
+    - tauto.
+    - destruct l.
+      + simpl; tauto.
+      + tauto.
+  Qed.
+
+  Fixpoint eval_or_list  (l : list A) :=
+    match l with
+    | nil => False
+    | e :: nil => eval e
+    | e1 ::l   => eval e1 \/ eval_or_list  l
+    end.
+
+  Fixpoint eval_or_list'  (l : list A) :=
+    match l with
+    | nil => False
+    | e1 ::l   => eval e1 \/ eval_or_list'  l
+    end.
+
+
+  Lemma eval_or_list_eq : forall l,
+      eval_or_list l <-> eval_or_list' l.
+  Proof.
+    induction l ; simpl.
+    - tauto.
+    - destruct l.
+      + simpl; tauto.
+      + tauto.
+  Qed.
+
+  Definition eval_op_list (o:lop) (l : list A) :=
+    match o with
+    | LAND => eval_and_list  l
+    | LOR  => eval_or_list  l
+    end.
+
+  Fixpoint eval_impl_list (l : list A) (r: Prop) :=
+    match l with
+    | nil => r
+    | e::l => eval e -> eval_impl_list l r
+    end.
+
+  Lemma eval_and_list_dec :
+    forall l,
+      Forall (fun x  => eval x \/ ~ eval x) l ->
+      eval_and_list  l \/  ~ eval_and_list l.
+  Proof.
+    intros. induction H.
+    - simpl. tauto.
+    - simpl.
+      destruct l. tauto.
+      tauto.
+  Qed.
+
+  Lemma eval_or_list_dec :
+    forall l,
+      Forall (fun x  => eval x \/ ~ eval x) l ->
+      eval_or_list  l \/  ~ eval_or_list l.
+  Proof.
+    intros. induction H.
+    - simpl. tauto.
+    - simpl.
+      destruct l. tauto. tauto.
+  Qed.
+
+  Lemma eval_op_list_dec :
+    forall o l,
+      Forall (fun x  => eval x \/ ~ eval x) l ->
+      eval_op_list o l \/  ~ eval_op_list o l.
+  Proof.
+    destruct o.
+    apply eval_and_list_dec.
+    apply eval_or_list_dec.
+  Qed.
+
+  Lemma eval_impl_list_dec :
+    forall l r,
+      Forall (fun x  => eval x \/ ~ eval x) l ->
+      r \/ ~ r ->
+      eval_impl_list l r \/  ~ eval_impl_list l r.
+  Proof.
+    intros l r H.
+    induction H.
+    - simpl. tauto.
+    - simpl.
+      intros.
+      tauto.
+  Qed.
+
+  Lemma eval_and_list'_Forall : forall l, eval_and_list' l <-> Forall eval l.
+  Proof.
+    induction l.
+    - simpl.
+      rewrite Forall_rew. tauto.
+    - simpl.
+      rewrite Forall_rew. tauto.
+  Qed.
+
+  Lemma eval_or_list'_Exists : forall l, eval_or_list' l <-> Exists eval l.
+  Proof.
+    induction l.
+    - simpl.
+      intuition. inversion H.
+    - simpl.
+      rewrite IHl ; intuition.
+      inv H1; tauto.
+  Qed.
+
+
+  Lemma eval_and_list_impl :
+    forall l l',
+      (forall x, In x l -> exists y, In y l' /\ (eval x <-> eval y)) ->
+      eval_and_list  l' -> eval_and_list  l.
+  Proof.
+    intros.
+    rewrite! eval_and_list_eq in *.
+    revert l' H H0.
+    induction l; simpl.
+    - intuition.
+    - intros.
+      split.
+      destruct (H a (or_introl eq_refl)).
+      destruct H1. rewrite H2.
+      clear H2.
+      revert x H1.
+      rewrite <- Forall_forall.
+      apply eval_and_list'_Forall in H0 ; auto.
+      eapply IHl ; eauto.
+  Qed.
+
+  Lemma eval_or_list_impl :
+    forall l l',
+      (forall x, In x l' -> exists y, In y l /\ (eval x <-> eval y)) ->
+      eval_or_list  l' -> eval_or_list  l.
+  Proof.
+    intros.
+    rewrite! eval_or_list_eq in *.
+    revert l H H0.
+    induction l'; simpl.
+    - tauto.
+    - intros.
+      destruct H0.
+      destruct (H a (or_introl eq_refl)).
+      destruct H1.
+      rewrite H2 in H0.
+      rewrite eval_or_list'_Exists.
+      rewrite Exists_exists.
+      exists x ; tauto.
+      eapply IHl' ; eauto.
+  Qed.
+
+  Lemma eval_and_list_app : forall l1 l2,
+      eval_and_list' (l1 ++ l2) <->  (eval_and_list' l1 /\ eval_and_list' l2).
+  Proof.
+    induction l1; simpl.
+    - tauto.
+    - intros. rewrite IHl1. tauto.
+  Qed.
+
+  Lemma eval_or_list_app : forall l1 l2,
+      eval_or_list' (l1 ++ l2) <->  (eval_or_list' l1 \/ eval_or_list' l2).
+  Proof.
+    induction l1; simpl.
+    - tauto.
+    - intros. rewrite IHl1. tauto.
+  Qed.
+
+  Lemma eval_and_list_rev_append : forall l1 l2,
+      eval_and_list' (rev_append l1 l2) <-> (eval_and_list' l1 /\ eval_and_list' l2).
+  Proof.
+    induction l1 ; simpl.
+    - tauto.
+    - intros.
+      rewrite IHl1. simpl.
+      tauto.
+  Qed.
+
+  Lemma eval_or_list_rev_append : forall l1 l2,
+      eval_or_list' (rev_append l1 l2) <-> (eval_or_list' l1 \/ eval_or_list' l2).
+  Proof.
+    induction l1 ; simpl.
+    - tauto.
+    - intros.
+      rewrite IHl1. simpl.
+      tauto.
+  Qed.
+
+  Definition eval_lop (o: lop) :=
+    match o with
+    | LAND => and
+    | LOR  => or
+    end.
+
+  Lemma eval_op_list_app : forall o l1 l2,
+      eval_op_list o (l1++l2) <->  eval_lop o (eval_op_list o l1) (eval_op_list o l2).
+  Proof.
+    destruct o; simpl;intros.
+    - rewrite! eval_and_list_eq.
+      rewrite eval_and_list_app.
+      tauto.
+    - rewrite! eval_or_list_eq.
+      rewrite eval_or_list_app.
+      tauto.
+  Qed.
+
+  Lemma eval_op_list_rev_append : forall o l1 l2,
+      eval_op_list o (rev_append l1 l2) <->  eval_lop o (eval_op_list o l1) (eval_op_list o l2).
+  Proof.
+    destruct o; simpl;intros.
+    - rewrite! eval_and_list_eq.
+      rewrite eval_and_list_rev_append.
+      tauto.
+    - rewrite! eval_or_list_eq.
+      rewrite eval_or_list_rev_append.
+      tauto.
+  Qed.
+
+  Lemma eval_op_list_cons : forall o e l,
+      eval_op_list o (e::l) <->  eval_lop o (eval e) (eval_op_list o l).
+  Proof.
+    destruct o; unfold eval_op_list; intros.
+    - rewrite! eval_and_list_eq.
+      simpl ; tauto.
+    - rewrite! eval_or_list_eq.
+      simpl ; tauto.
+  Qed.
+
+  Lemma eval_impl_list_eq : forall l (r:Prop),
+      (eval_and_list l -> r)
+      <-> eval_impl_list l r.
+  Proof.
+    intros.
+    rewrite eval_and_list_eq.
+    induction l; simpl.
+    - tauto.
+    - tauto.
+  Qed.
+
+  Lemma eval_impl_list_iff : forall l r l' r',
+      (eval_and_list l <-> eval_and_list l') ->
+      (r <->  r') ->
+      eval_impl_list l r <-> eval_impl_list l' r'.
+  Proof.
+    intros.
+    rewrite <- ! eval_impl_list_eq.
+    rewrite! eval_and_list_eq in *.
+    tauto.
+  Qed.
+
+  Lemma eval_and_list_rev : forall l,
+      eval_and_list'  (rev l) <-> eval_and_list'  l.
+  Proof.
+    induction l; simpl.
+    - tauto.
+    - rewrite eval_and_list_app.
+      simpl. tauto.
+  Qed.
+
+  Lemma eval_or_list_rev : forall l,
+      eval_or_list'  (rev l) <-> eval_or_list'  l.
+  Proof.
+    induction l; simpl.
+    - tauto.
+    - rewrite eval_or_list_app.
+      simpl. tauto.
+  Qed.
+
+
+End EvalList.
+
+Definition clause := list Lit.t.
+
+Definition wf (l : clause) :=
+  exists l1 l2, l=(List.map NEG l1) ++ (List.map POS l2).
+
+Fixpoint eval_clause (env : HFormula -> Prop) (cl : clause) :=
+  match cl with
+  | nil => False
+  | e::cl' => eval_lit env e (eval_clause env cl')
+  end.
+
+Fixpoint beval_clause (env : HFormula -> bool) (cl : clause) :=
+  match cl with
+  | nil => false
+  | e::cl' => beval_lit env e || beval_clause env cl'
+  end.
+
+Definition cnf := list clause.
+
+Definition penv (env : HFormula -> bool) := fun x => is_true (env x).
+
+Definition beval_cnf (env :HFormula -> bool) (l: cnf) :=
+  List.fold_right (fun e acc => beval_clause env e && acc) true l.
+
+Definition eval_cnf (env :HFormula -> Prop) (l: cnf) :=
+  List.fold_right (fun e acc => eval_clause env e /\ acc) True l.
+
+
+Lemma beval_clause_app : forall env l1 l2,
+    beval_clause env (l1 ++ l2) = (beval_clause env l1 || beval_clause env l2).
+Proof.
+  induction l1; simpl.
+  - reflexivity.
+  - intros.
+    rewrite IHl1.
+    btauto.
+Qed.
+
+Lemma beval_cnf_app : forall env l1 l2,
+    beval_cnf env (l1 ++ l2) = (beval_cnf env l1 && beval_cnf env l2).
+Proof.
+  induction l1; simpl.
+  - tauto.
+  - intros.
+    rewrite IHl1.
+    btauto.
+Qed.
+
+Lemma eval_cnf_app : forall env l1 l2,
+    eval_cnf env (l1 ++ l2) <-> (eval_cnf env l1 /\ eval_cnf env l2).
+Proof.
+  induction l1; simpl.
+  - tauto.
+  - intros.
+    rewrite IHl1.
+    tauto.
+Qed.
