theories/Lit.v
@@ -1,0 +1,253 @@
+(* Copyright 2023 Frédéric Besson <frederic.besson@inria.fr> *)
+Require Import Bool ZifyBool ZArith ZifyUint63 Uint63 Lia List.
+Require Import Morphisms.
+Require Import Cdcl.Lib Cdcl.Syntax.
+
+(* Here, we consider [HFormula] as tokens. *)
+
+
+  Section HEQB.
+    Variable eqb : LForm -> LForm -> bool.
+
+    Definition xhformula_eqb (f1 f2: HFormula) :=
+      HCons.eq_hc f1 f2 && eqb f1.(HCons.elt) f2.(HCons.elt).
+  End HEQB.
+
+  Fixpoint formula_eqb (f1 f2 : LForm) {struct f1}: bool :=
+    match f1 , f2 with
+    | LAT i , LAT j => Uint63.eqb i j
+    | LOP o1 l1, LOP o2 l2 => lop_eqb o1 o2 && forall2b (xhformula_eqb formula_eqb) l1 l2
+    | LIMPL l1 r1, LIMPL l2 r2 => forall2b (xhformula_eqb formula_eqb) l1 l2 && xhformula_eqb formula_eqb r1 r2
+    | _ , _ => false
+    end.
+
+  Definition hformula_eqb (x y: HFormula) := xhformula_eqb formula_eqb x y.
+
+  Fixpoint formula_eqb_true (f1 f2: LForm) : formula_eqb f1 f2 = true -> f1 = f2.
+  Proof.
+    assert (REC : forall f1 f2, xhformula_eqb formula_eqb f1 f2 = true -> f1 = f2).
+    {
+      unfold xhformula_eqb.
+      intros.
+      destruct f0,f3 ; simpl in *.
+      unfold HCons.eq_hc in H.
+      simpl in *. rewrite! andb_true_iff in H.
+      destruct H. destruct H.
+      f_equal;auto. lia. rewrite eqb_true_iff in H1; auto.
+    }
+    assert (ALL : forall l1 l2,
+               forall2b (xhformula_eqb formula_eqb) l1 l2 = true ->
+               l1 = l2).
+    {
+      intros.
+      apply forall2b_Forall2 in H.
+      revert l2 H.
+      induction l1.
+      - intros. inv H. reflexivity.
+      - intros.
+        inv H. apply IHl1 in H4.
+        apply REC in H2.
+        congruence.
+    }
+    destruct f1 ; simpl; destruct f2; simpl; try congruence.
+    - intros. f_equal. lia.
+    - intros.
+      rewrite andb_true_iff in *.
+      destruct H.
+      apply lop_eqb_true in H.
+      f_equal. auto. apply ALL; auto.
+    - intros.
+      rewrite andb_true_iff in *.
+      destruct H.
+      f_equal ;auto.
+  Qed.
+
+  Fixpoint formula_eqb_refl (f1: LForm) : formula_eqb f1 f1 = true.
+  Proof.
+    assert (REC : forall f1, xhformula_eqb formula_eqb f1 f1 = true).
+    {
+      unfold xhformula_eqb.
+      intros.
+      destruct f0 ; simpl in *.
+      unfold HCons.eq_hc.
+      simpl. rewrite! andb_true_iff.
+      split_and. lia.
+      apply eqb_reflx.
+      apply formula_eqb_refl.
+    }
+    assert (ALL : forall l1,
+               forall2b (xhformula_eqb formula_eqb) l1 l1 = true).
+    {
+      intros.
+      induction l1.
+      - reflexivity.
+      -  simpl.
+         rewrite REC. rewrite IHl1.
+         reflexivity.
+    }
+    destruct f1 ; simpl; try congruence.
+    - lia.
+    - rewrite andb_true_iff.
+      split_and.
+      apply lop_eqb_refl.
+      apply ALL;auto.
+    - intros.
+      rewrite andb_true_iff in *.
+      split;
+      auto.
+  Qed.
+
+
+
+  Definition hformula_eqb_true (f1 f2: HFormula) : hformula_eqb f1 f2 = true -> f1 = f2.
+  Proof.
+    unfold hformula_eqb.
+    {
+      unfold xhformula_eqb.
+      intros.
+      destruct f1,f2 ; simpl in *.
+      unfold HCons.eq_hc in H.
+      simpl in *. rewrite! andb_true_iff in H.
+      destruct H. destruct H.
+      f_equal;auto. lia. rewrite eqb_true_iff in H1; auto.
+      apply formula_eqb_true; auto.
+    }
+  Qed.
+
+
+  Lemma hformula_eqb_refl (f1: HFormula) : hformula_eqb f1 f1 = true.
+  Proof.
+    unfold hformula_eqb.
+    destruct f1 ; simpl in *.
+    unfold xhformula_eqb.
+    unfold HCons.eq_hc. simpl.
+    rewrite! andb_true_iff.
+    split_and. lia.
+    apply eqb_reflx.
+    apply formula_eqb_refl.
+  Qed.
+
+  Lemma hformula_eq_dec (f1 f2: HFormula) : {f1 = f2} + {f1 <> f2}.
+  Proof.
+    destruct (hformula_eqb f1 f2) eqn:HF.
+    apply hformula_eqb_true in HF.
+    left ; auto.
+    right. intro. subst. rewrite hformula_eqb_refl in HF.  discriminate.
+  Qed.
+
+Definition t := literal.
+
+Definition pol (x:t) :=
+  match x with
+  | POS _ => true
+  | NEG _ => false
+  end.
+
+Definition isPOS (x:t) :=
+  pol x = true.
+
+
+Definition var (x:t) :=
+  match x with
+  | POS p => p
+  | NEG p => p
+  end.
+
+Definition neg (x:t) :=
+  match x with
+  | POS x => NEG x
+  | NEG x => POS x
+  end.
+
+
+Definition beval_lit (env : HFormula -> bool) (l:t) :=
+  if pol l then env (var l) else
+    negb (env (var l)).
+
+Definition eval_lit (env: HFormula -> Prop) (l:t) (X:Prop)  :=
+  if pol l then env (var l) \/ X
+  else env (var l) -> X.
+
+Lemma beval_lit_neg : forall env l,
+    beval_lit env l = negb (beval_lit env (neg l)).
+Proof.
+  unfold beval_lit.
+  destruct l; simpl; auto.
+  rewrite negb_involutive. reflexivity.
+Qed.
+
+
+Add Parametric Morphism (env:HFormula -> Prop) (l:t) : (eval_lit env l) with signature iff ==> iff as eval_lit_morph.
+Proof.
+  unfold eval_lit.
+  intros.
+  destruct (pol l). tauto.
+  tauto.
+Qed.
+
+Definition get_pol (p:HFormula) (l : Lit.t) : option bool :=
+  if hformula_eqb p (var l) then Some (pol l) else None.
+
+
+Definition eq_dec (l1 l2:t) : {l1 = l2} + {l1 <> l2}.
+Proof.
+  decide equality.
+  apply hformula_eq_dec.
+  apply hformula_eq_dec.
+Qed.
+
+
+Definition make (b:bool) (v:HFormula) :=
+  if b then POS v else NEG v.
+
+Lemma var_make : forall b v, var (make b v) = v.
+Proof.
+  unfold make. destruct b;reflexivity.
+Qed.
+
+Lemma decomp : forall l,
+    l = (if pol l then POS (var l) else NEG (var l)).
+Proof.
+  destruct l; reflexivity.
+Qed.
+
+Lemma get_pol_inv : forall p l b,
+    get_pol p l = Some b -> l = make b p.
+Proof.
+  unfold get_pol.
+  intros.
+  destruct (hformula_eqb p (var l)) eqn:E.
+  inv H.
+  apply hformula_eqb_true in E.
+  subst.
+  apply decomp.
+  discriminate.
+Qed.
+
+Lemma get_pol_None : forall p l,
+    get_pol p l = None -> var l <> p.
+Proof.
+  unfold get_pol.
+  intros.
+  destruct (hformula_eqb p (var l)) eqn:E.
+  discriminate.
+  intro. subst.
+  rewrite hformula_eqb_refl in E. discriminate.
+Qed.
+
+Lemma eval_lit_negb_make : forall env b p,
+    beval_lit env (make b p) = negb (beval_lit env (make (negb b) p)).
+Proof.
+  unfold beval_lit. unfold make.
+  destruct b; simpl;auto.
+  intros. rewrite negb_involutive. reflexivity.
+Qed.
+
+Lemma make_var : forall b a,
+    make b (var a) <> a -> make (negb b) (var a) = a.
+Proof.
+  unfold make.
+  destruct b,a; simpl; congruence.
+Qed.
+
+
