theories/Syntax.v
@@ -1,0 +1,103 @@
+(* Copyright 2023 Frédéric Besson <frederic.besson@inria.fr> *)
+Require Import Bool Uint63.
+
+Module HCons.
+  (* The [HCons] module allows to tag a term with
+      - a unique identifier [id]
+      - a boolean stating whether the term is decidable
+   *)
+  Section S.
+    Variable A: Type.
+
+    Record t : Type :=
+      mk {
+          id : int;
+          is_dec: bool;
+          elt: A
+        }.
+
+
+    Lemma dest_eq : forall f,
+        mk (id f) (is_dec f) (elt f) = f.
+    Proof.
+      destruct f ; reflexivity.
+    Qed.
+
+    Definition eq_hc (f1 f2 : t) := (id f1 =? id f2)%uint63 && Bool.eqb (is_dec f1) (is_dec f2).
+
+
+  End S.
+
+  Definition map [A B] (f: A -> B) (e: t A) : t B :=
+    mk _ (id _ e) (is_dec _ e) (f (elt _ e)).
+
+End HCons.
+Arguments HCons.mk {A} id is_dec elt.
+Arguments HCons.elt {A} .
+Arguments HCons.id {A} .
+Arguments HCons.is_dec {A} .
+Arguments HCons.eq_hc {A}.
+
+(* [BForm] stands for boolean formula.
+   This provides the surface of formulae.
+   The formulae are either interpreted over [bool] or [Prop].
+ *)
+
+Inductive op :=
+| NOT | AND | OR | IMPL | IFF (i1 i2:int).
+
+Inductive bprop := EQB (i1 i2:int).
+
+Inductive ite := ITE (i1 i2:int).
+
+Inductive kind : Type :=
+|IsProp
+|IsBool.
+
+Inductive BForm  : kind -> Type :=
+| BTT   : forall (k: kind), BForm k
+| BFF   : forall (k: kind), BForm k
+| BAT   : forall (k: kind), int -> BForm k
+| BOP   : forall (k: kind), op -> HCons.t (BForm k) ->
+                            HCons.t (BForm k) -> BForm k
+| BITE  : forall (k:kind), ite -> HCons.t (BForm IsBool) -> HCons.t (BForm k) ->
+                           HCons.t (BForm k) -> BForm k
+| BPROP   : bprop -> HCons.t (BForm IsBool) -> HCons.t (BForm IsBool) -> BForm IsProp
+.
+
+(** [LForm] is the desuggared syntax for formulae.
+      The operators take a list of formulae *)
+
+Inductive lop := LAND | LOR.
+
+Inductive LForm : Type :=
+| LAT : int -> LForm
+| LOP : lop -> list (HCons.t LForm) -> LForm
+| LIMPL : list (HCons.t LForm) ->  (HCons.t LForm)  -> LForm.
+
+Definition HFormula : Type := HCons.t LForm.
+
+(** A [literal] is either a positive or negative formula.
+    A clause is a list of literals. *)
+Inductive literal : Type :=
+| POS (f:HFormula)
+| NEG (f:HFormula).
+
+Definition lop_eqb (o o': lop) : bool :=
+  match o , o' with
+  | LAND , LAND => true
+  | LOR  , LOR  => true
+  | _ , _ => false
+  end.
+
+Lemma lop_eqb_true : forall o o',
+    lop_eqb o o' = true -> o = o'.
+Proof.
+  destruct o,o' ; simpl ; intuition congruence.
+Qed.
+
+Lemma lop_eqb_refl : forall l,
+    lop_eqb l l = true.
+Proof.
+  destruct l;reflexivity.
+Qed.
